cedar-lean/Cedar/Data/Map.lean
@@ -14,7 +14,11 @@
  limitations under the License.
 -/
 
-import Cedar.Data.Set
+module
+
+public import Cedar.Data.List
+public import Cedar.Data.Set
+
 /-!
 
 This file defines a simple map data types, backed by a sorted duplicate-free
@@ -27,94 +31,94 @@ Use `Map.make` to construct well-formed maps from lists of key-value pairs.
 
 namespace Cedar.Data
 
-inductive Map (α : Type u) (β : Type v) where
+public inductive Map (α : Type u) (β : Type v) where
 | mk : List (α × β) -> Map α β
 deriving Repr, DecidableEq, Inhabited
 
 namespace Map
 
-abbrev kvs  {α : Type u} {β : Type v} (m : Map α β) := m.1
+public abbrev kvs  {α : Type u} {β : Type v} (m : Map α β) := m.1
 
 ----- Definitions -----
 
 /-- Creates a well-formed map from the given list of pairs. -/
-def make {α β} [LT α] [DecidableLT α] (kvs : List (α × β)) : Map α β :=
+public def make {α β} [LT α] [DecidableLT α] (kvs : List (α × β)) : Map α β :=
   Map.mk (kvs.canonicalize Prod.fst)
 
 /-- Empty map -/
-def empty {α β} : Map α β := .mk []
+public def empty {α β} : Map α β := .mk []
 
 /-- Returns an ordered and duplicate free list provided the given map is well-formed. -/
-def toList {α : Type u} {β : Type v} (m : Map α β) : List (Prod α β) := m.kvs
+public def toList {α : Type u} {β : Type v} (m : Map α β) : List (Prod α β) := m.kvs
 
 
 /-- Returns the keys of `m` as a set. -/
-def keys {α β} (m : Map α β) : Set α :=
+public def keys {α β} (m : Map α β) : Set α :=
   Set.mk (m.kvs.map Prod.fst) -- well-formed by construction
 
 /-- Returns the values of `m` as a list. -/
-def values {α β} (m : Map α β) : List β :=
+public def values {α β} (m : Map α β) : List β :=
   m.kvs.map Prod.snd
 
 /-- Returns the binding for `k` in `m`, if any. -/
-def find? {α β} [BEq α] (m : Map α β) (k : α) : Option β :=
+public def find? {α β} [BEq α] (m : Map α β) (k : α) : Option β :=
   match m.kvs.find? (λ ⟨k', _⟩ => k' == k) with
   | some (_, v) => some v
   | _           => none
 
 /-- Returns true if `m` contains a mapping for the key `k`. -/
-def contains {α β} [BEq α] (m : Map α β) (k : α) : Bool :=
+public def contains {α β} [BEq α] (m : Map α β) (k : α) : Bool :=
   (m.find? k).isSome
 
 /-- Returns the binding for `k` in `m` or `err` if none is found. -/
-def findOrErr {α β ε} [BEq α] (m : Map α β) (k : α) (err: ε) : Except ε β :=
+public def findOrErr {α β ε} [BEq α] (m : Map α β) (k : α) (err: ε) : Except ε β :=
   match m.find? k with
   | some v => .ok v
   | _      => .error err
 
 /-- Returns the binding for `k` in `m`, or panics if none is found. -/
-def find! {α β} [Repr α] [BEq α] [Inhabited β] (m : Map α β) (k : α) : β :=
+public def find! {α β} [Repr α] [BEq α] [Inhabited β] (m : Map α β) (k : α) : β :=
   match m.find? k with
   | some v => v
   | _      => panic! s!"find!: key {repr k} not found"
 
 /-- Filters `m` using `f`. -/
-def filter {α β} (f : α → β → Bool) (m : Map α β) : Map α β :=
+public def filter {α β} (f : α → β → Bool) (m : Map α β) : Map α β :=
   Map.mk (m.kvs.filter (λ ⟨k, v⟩ => f k v))
 
-def size {α β} (m : Map α β) : Nat :=
+public def size {α β} (m : Map α β) : Nat :=
   m.kvs.length
 
-def mapOnValues {α β γ} (f : β → γ) (m : Map α β) : Map α γ :=
+public def mapOnValues {α β γ} (f : β → γ) (m : Map α β) : Map α γ :=
   Map.mk (m.kvs.map (λ (k, v) => (k, f v)))
 
-def mapOnKeys {α β γ} [LT γ] [DecidableLT γ] (f : α → γ) (m : Map α β) : Map γ β :=
+public def mapOnKeys {α β γ} [LT γ] [DecidableLT γ] (f : α → γ) (m : Map α β) : Map γ β :=
   Map.make (m.kvs.map (λ (k, v) => (f k, v)))
 
-def mapMOnValues {α β γ} [LT α] [DecidableLT α] [Monad m] (f : β → m γ) (map : Map α β) : m (Map α γ) := do
+public def mapMOnValues {α β γ} [LT α] [DecidableLT α] [Monad m] (f : β → m γ) (map : Map α β) : m (Map α γ) := do
   let kvs ← map.kvs.mapM (λ (k, v) => f v >>= λ v' => pure (k, v'))
   pure (Map.mk kvs)
 
-def mapMOnKeys {α β γ} [LT γ] [DecidableLT γ] [Monad m] (f : α → m γ) (map : Map α β) : m (Map γ β) := do
+public def mapMOnKeys {α β γ} [LT γ] [DecidableLT γ] [Monad m] (f : α → m γ) (map : Map α β) : m (Map γ β) := do
   let kvs ← map.kvs.mapM (λ (k, v) => f k >>= λ k' => pure (k', v))
   pure (Map.make kvs)
 
-def wellFormed {α β} [LT α] [DecidableLT α] (m : Map α β) : Bool :=
+public def wellFormed {α β} [LT α] [DecidableLT α] (m : Map α β) : Bool :=
   m.toList.isSortedBy Prod.fst
 
 ----- Instances -----
 
-instance [LT (Prod α β)] : LT (Map α β) where
+public instance [LT (Prod α β)] : LT (Map α β) where
   lt a b := a.kvs < b.kvs
 
-instance decLt [LT (Prod α β)] [DecidableEq (Prod α β)] [DecidableLT (Prod α β)] : (n m : Map α β) → Decidable (n < m)
+public instance decLt [LT (Prod α β)] [DecidableEq (Prod α β)] [DecidableLT (Prod α β)] : (n m : Map α β) → Decidable (n < m)
   | .mk nkvs, .mk mkvs => List.decidableLT nkvs mkvs
 
 -- enables ∈ notation for map keys
-instance : Membership α (Map α β) where
+public instance : Membership α (Map α β) where
   mem m a := List.Mem a (m.kvs.map Prod.fst)
 
-instance [LT α] [DecidableLT α] : HAppend (Map α β) (Map α β) (Map α β) where
+public instance [LT α] [DecidableLT α] : HAppend (Map α β) (Map α β) (Map α β) where
   hAppend a b := Map.make (a.kvs ++ b.kvs)
 
 end Map
