cedar-lean/Cedar/Thm/Data/Control.lean
@@ -14,65 +14,65 @@
  limitations under the License.
 -/
 
+module
 
 /-!
 This file contains `simp` lemmas for proofs about code that uses the `do`
 notation together with `Except` and `Option`.
 -/
 
-
 -- The `Except.bind_*` theorems let `simp` reduce terms that use the `do` notation.
-@[simp] theorem Except.bind_ok_T (a : α) (f : α → ExceptT ε Id β) :
+@[simp] public theorem Except.bind_ok_T (a : α) (f : α → ExceptT ε Id β) :
   (bind (Except.ok a) f : ExceptT ε Id β) = f a
 := by rfl
 
-@[simp] theorem Except.bind_ok (a : α) (f : α → Except ε β) :
+@[simp] public theorem Except.bind_ok (a : α) (f : α → Except ε β) :
   (bind (Except.ok a) f : Except ε β) = f a
 := by rfl
 
-@[simp] theorem Except.bind_err (e : ε) (f : α → Except ε β) :
+@[simp] public theorem Except.bind_err (e : ε) (f : α → Except ε β) :
   (bind (Except.error e) f : Except ε β) = (Except.error e)
 := by rfl
 
 -- The `Option.bind_*` theorems let `simp` reduce terms that use the `do` notation.
-@[simp] theorem Option.bind_some_T (a : α) (f : α → OptionT Id β) :
+@[simp] public theorem Option.bind_some_T (a : α) (f : α → OptionT Id β) :
   (bind (Option.some a) f : OptionT Id β) = f a
 := by rfl
 
-@[simp] theorem Option.bind_some_fun (a : α) (f : α → Option β) :
+@[simp] public theorem Option.bind_some_fun (a : α) (f : α → Option β) :
   (bind (Option.some a) f : Option β) = f a
 := by rfl
 
-@[simp] theorem Option.bind_none_fun (f : α → Option β) :
+@[simp] public theorem Option.bind_none_fun (f : α → Option β) :
   (bind Option.none f : Option β) = Option.none
 := by rfl
 
-theorem do_some {opt : Option α} {f : α → β} :
+public theorem do_some {opt : Option α} {f : α → β} :
   (do let v ← opt ; some (f v)) = some b ↔
   ∃ a, opt = some a ∧ f a = b
 := by cases opt <;> simp
 
-theorem do_error {res : Except ε α} {e : ε} {f : α → β} :
+public theorem do_error {res : Except ε α} {e : ε} {f : α → β} :
   (do let v ← res ; .ok (f v)) = .error e ↔
   res = .error e
 := by cases res <;> simp
 
-theorem do_ok_eq_ok {res : Except ε α} {f : α → β} :
+public theorem do_ok_eq_ok {res : Except ε α} {f : α → β} :
   (do let v ← res ; .ok (f v)) = .ok b ↔
   ∃ a, res = .ok a ∧ f a = b
 := by cases res <;> simp
 
-theorem do_eq_ok {res : Except ε α} {f : α → Except ε β} :
+public theorem do_eq_ok {res : Except ε α} {f : α → Except ε β} :
   (do let v ← res ; f v) = .ok b ↔
   ∃ a, res = .ok a ∧ f a = .ok b
 := by cases res <;> simp
 
-theorem do_eq_ok₂ {res₁ res₂: Except ε PUnit} :
+public theorem do_eq_ok₂ {res₁ res₂: Except ε PUnit} :
   (do res₁ ; res₂) = .ok () → res₁ = .ok () ∧ res₂ = .ok ()
 := by
   cases res₁ <;> cases res₂ <;> simp
 
-theorem to_option_some {v : α} {res: Except ε α} :
+public theorem to_option_some {v : α} {res: Except ε α} :
   res.toOption = .some v ↔ res = .ok v
 := by
   constructor
@@ -86,7 +86,7 @@ theorem to_option_some {v : α} {res: Except ε α} :
     intro h
     simp only [Except.toOption, h]
 
-theorem to_option_none {res: Except ε α} :
+public theorem to_option_none {res: Except ε α} :
   res.toOption = .none → (∃ err, res = .error err)
 := by
   intro h
@@ -95,7 +95,7 @@ theorem to_option_none {res: Except ε α} :
   rename_i err
   exists err
 
-theorem to_option_left_ok {α ε₁ ε₂} {v : α} {res₁ : Except ε₁ α} {res₂ : Except ε₂ α} :
+public theorem to_option_left_ok {α ε₁ ε₂} {v : α} {res₁ : Except ε₁ α} {res₂ : Except ε₂ α} :
   res₁.toOption = res₂.toOption → res₁ = .ok v → res₂ = .ok v
 := by
   intro h₀ h₁
@@ -108,14 +108,14 @@ theorem to_option_left_ok {α ε₁ ε₂} {v : α} {res₁ : Except ε₁ α} {
   · cases h₀
   · cases h₁
 
-theorem to_option_right_ok {α ε₁ ε₂} {v : α} {res₁ : Except ε₁ α} {res₂ : Except ε₂ α} :
+public theorem to_option_right_ok {α ε₁ ε₂} {v : α} {res₁ : Except ε₁ α} {res₂ : Except ε₂ α} :
   res₁.toOption = res₂.toOption → res₂ = .ok v → res₁ = .ok v
 := by
   intro h
   symm at h
   exact to_option_left_ok h
 
-theorem to_option_right_ok' {α ε₁ ε₂} {v : α} {res₁ : Except ε₁ α} :
+public theorem to_option_right_ok' {α ε₁ ε₂} {v : α} {res₁ : Except ε₁ α} :
   res₁.toOption = ((.ok v) : Except ε₂ α).toOption → res₁ = Except.ok v
 := by
   generalize h : ((.ok v) : Except ε₂ α) = res₂
@@ -123,14 +123,14 @@ theorem to_option_right_ok' {α ε₁ ε₂} {v : α} {res₁ : Except ε₁ α}
   intro h₁
   exact to_option_right_ok h₁ h
 
-theorem to_option_left_ok' {α ε₁ ε₂} {v : α} {res₂ : Except ε₂ α} :
+public theorem to_option_left_ok' {α ε₁ ε₂} {v : α} {res₂ : Except ε₂ α} :
   ((.ok v) : Except ε₁ α).toOption = res₂.toOption → res₂ = Except.ok v
 := by
   intro h
   symm at h
   exact to_option_right_ok' h
 
-theorem to_option_left_err {ε₁ ε₂ α} {err₁: ε₁} {res₂ : Except ε₂ α} :
+public theorem to_option_left_err {ε₁ ε₂ α} {err₁: ε₁} {res₂ : Except ε₂ α} :
   (Except.error err₁).toOption = res₂.toOption → ∃ err₂, res₂ = .error err₂
 := by
   intro h
@@ -139,14 +139,14 @@ theorem to_option_left_err {ε₁ ε₂ α} {err₁: ε₁} {res₂ : Except ε�
   · cases h
   · simp only [Except.error.injEq, exists_eq']
 
-theorem to_option_right_err {ε₂ ε₁ α} {err₂: ε₂} {res₁ : Except ε₁ α} :
+public theorem to_option_right_err {ε₂ ε₁ α} {err₂: ε₂} {res₁ : Except ε₁ α} :
   res₁.toOption = (Except.error err₂).toOption → ∃ err₁, res₁ = .error err₁
 := by
   intro h
   symm at h
   exact to_option_left_err h
 
-theorem do_error_to_option {res : Except ε α} {e : ε} :
+public theorem do_error_to_option {res : Except ε α} {e : ε} :
   (do let (_ : α) ← res ; (.error e : Except ε α)).toOption = .none
 := by
   cases res <;> simp [Except.toOption]
