cedar-lean/Cedar/Thm/Data/List/Canonical.lean
@@ -14,7 +14,11 @@
  limitations under the License.
 -/
 
-import Cedar.Thm.Data.List.Basic
+module
+
+public import Cedar.Data.List
+import all Cedar.Data.List -- in this module, we allow unfolding definitions in Cedar.Data.List, not (only) using lemmas defined in the imports below
+public import Cedar.Thm.Data.List.Basic
 
 /-!
 
@@ -30,11 +34,11 @@ open Cedar.Data
 
 /-! ### insertCanonical -/
 
-theorem insertCanonical_singleton [LT β] [DecidableLT β] (f : α → β)  (x : α) :
+public theorem insertCanonical_singleton [LT β] [DecidableLT β] (f : α → β)  (x : α) :
   insertCanonical f x [] = [x]
 := by unfold insertCanonical; rfl
 
-theorem insertCanonical_not_nil [DecidableEq β] [LT β] [DecidableLT β] (f : α → β) (x : α) (xs : List α) :
+public theorem insertCanonical_not_nil [DecidableEq β] [LT β] [DecidableLT β] (f : α → β) (x : α) (xs : List α) :
   insertCanonical f x xs ≠ []
 := by
   unfold insertCanonical
@@ -46,7 +50,7 @@ theorem insertCanonical_not_nil [DecidableEq β] [LT β] [DecidableLT β] (f : �
     split at h <;> try trivial
     split at h <;> trivial
 
-theorem insertCanonical_mem [LT β] [Cedar.Data.StrictLT β] [DecidableLT β]
+public theorem insertCanonical_mem [LT β] [Cedar.Data.StrictLT β] [DecidableLT β]
   {f : α → β} {xs : List α} (x : α) :
   x ∈ List.insertCanonical f x xs
 := by
@@ -58,7 +62,7 @@ theorem insertCanonical_mem [LT β] [Cedar.Data.StrictLT β] [DecidableLT β]
     split; any_goals simp
     apply Or.inr ih
 
-theorem insertCanonical_find?
+public theorem insertCanonical_find?
   [LT β] [Cedar.Data.StrictLT β] [DecidableLT β] [BEq β] [LawfulBEq β]
   {f : α → β} {xs : List α} (x : α) :
   (List.insertCanonical f x xs).find? (λ e => f e == f x) = x
@@ -110,7 +114,39 @@ theorem insertCanonical_preserves_non_duplicate_element
         cases hltgt <;> contradiction
       case _ hy => simp [hy]
 
-theorem insertCanonical_sortedBy [LT β] [StrictLT β] [DecidableLT β] {f : α → β} {xs : List α} (x : α) :
+public theorem insertCanonical_preserves_find_other_element
+  [LT α] [DecidableLT α] [BEq α] [StrictLT α]
+  (k : α)
+  (x : (α × β)) (xs : List (α × β))  :
+  (x.fst == k) = false →
+  (List.insertCanonical Prod.fst x xs).find? (λ x => x.fst == k) =
+  xs.find? (λ x => x.fst == k)
+:= by
+  intro h₁
+  unfold List.insertCanonical
+  split
+  . simp
+    assumption
+  . simp
+    split
+    . simp [List.find?]
+      rw [h₁]
+    . split
+      . unfold List.find?
+        rename_i tl h₂ h₃
+        have ih := insertCanonical_preserves_find_other_element k x tl h₁
+        rw [ih]
+      . unfold List.find?
+        rw [h₁]
+        simp
+        rename_i hd₂ tl₂ h₂ h₃
+        rename LT α => i₁
+        rename StrictLT α => i₂
+        have h₄ := @StrictLT.if_not_lt_gt_then_eq α i₁ i₂ x.fst hd₂.fst h₂ h₃
+        rw [← h₄]
+        rw [h₁]
+
+public theorem insertCanonical_sortedBy [LT β] [StrictLT β] [DecidableLT β] {f : α → β} {xs : List α} (x : α) :
   SortedBy f xs →
   SortedBy f (insertCanonical f x xs)
 := by
@@ -166,7 +202,7 @@ theorem insertCanonical_cases [LT β] [DecidableLT β] (f : α → β) (x y : α
     case pos _ _ h₃ => simp [h₃, h₁]
     case neg _ _ h₃ => simp [h₃]
 
-theorem insertCanonical_subset [LT β] [DecidableLT β] (f : α → β) (x : α) (xs : List α) :
+public theorem insertCanonical_subset [LT β] [DecidableLT β] (f : α → β) (x : α) (xs : List α) :
   insertCanonical f x xs ⊆ x :: xs
 := by
   induction xs
@@ -181,7 +217,7 @@ theorem insertCanonical_subset [LT β] [DecidableLT β] (f : α → β) (x : α)
     · simp only [h₁, cons_subset, mem_cons, true_or, true_and]
       exact Subset.trans (List.subset_cons_self hd tl) (List.subset_cons_self x (hd :: tl))
 
-theorem insertCanonical_equiv [LT α] [StrictLT α] [DecidableLT α] (x : α) (xs : List α) :
+public theorem insertCanonical_equiv [LT α] [StrictLT α] [DecidableLT α] (x : α) (xs : List α) :
   x :: xs ≡ insertCanonical id x xs
 := by
   unfold insertCanonical
@@ -237,7 +273,7 @@ theorem insertCanonical_equiv [LT α] [StrictLT α] [DecidableLT α] (x : α) (x
               apply cons_equiv_cons
               exact ih
 
-theorem insertCanonical_preserves_forallᵥ {α β γ} [LT α] [StrictLT α] [DecidableLT α] {p : β → γ → Prop}
+public theorem insertCanonical_preserves_forallᵥ {α β γ} [LT α] [StrictLT α] [DecidableLT α] {p : β → γ → Prop}
   {kv₁ : α × β} {kv₂ : α × γ} {kvs₁ : List (α × β)} {kvs₂ : List (α × γ)}
   (h₁ : kv₁.fst = kv₂.fst ∧ p kv₁.snd kv₂.snd)
   (h₂ : Forallᵥ p kvs₁ kvs₂) :
@@ -266,7 +302,7 @@ theorem insertCanonical_preserves_forallᵥ {α β γ} [LT α] [StrictLT α] [De
       · contradiction
       · exact Forall₂.cons (by exact h₁) (by exact h₄)
 
-theorem insertCanonical_map_fst {α β γ} [LT α] [StrictLT α] [DecidableLT α] (xs : List (α × β)) (f : β → γ) (x : α × β) :
+public theorem insertCanonical_map_fst {α β γ} [LT α] [StrictLT α] [DecidableLT α] (xs : List (α × β)) (f : β → γ) (x : α × β) :
   insertCanonical Prod.fst (Prod.map id f x) (map (Prod.map id f) xs) =
   map (Prod.map id f) (insertCanonical Prod.fst x xs)
 := by
@@ -282,7 +318,7 @@ theorem insertCanonical_map_fst {α β γ} [LT α] [StrictLT α] [DecidableLT α
         simp [ih, Prod.map]
       · simp [Prod.map]
 
-theorem insertCanonical_map_fst_canonicalize {α β γ} [LT α] [StrictLT α] [DecidableLT α] (xs : List (α × β)) (f : β → γ) (x : α × β) :
+public theorem insertCanonical_map_fst_canonicalize {α β γ} [LT α] [StrictLT α] [DecidableLT α] (xs : List (α × β)) (f : β → γ) (x : α × β) :
   insertCanonical Prod.fst (Prod.map id f x) (canonicalize Prod.fst (map (Prod.map id f) xs)) =
   map (Prod.map id f) (insertCanonical Prod.fst x (canonicalize Prod.fst xs))
 := by
@@ -294,11 +330,11 @@ theorem insertCanonical_map_fst_canonicalize {α β γ} [LT α] [StrictLT α] [D
 
 /-! ## canonicalize -/
 
-theorem canonicalize_nil [LT β] [DecidableLT β] (f : α → β) :
+public theorem canonicalize_nil [LT β] [DecidableLT β] (f : α → β) :
   canonicalize f [] = []
 := by unfold canonicalize; rfl
 
-theorem canonicalize_nil' [DecidableEq β] [LT β] [DecidableLT β] (f : α → β) (xs : List α) :
+public theorem canonicalize_nil' [DecidableEq β] [LT β] [DecidableLT β] (f : α → β) (xs : List α) :
   xs = [] ↔ (canonicalize f xs) = []
 := by
   constructor
@@ -315,7 +351,7 @@ theorem canonicalize_nil' [DecidableEq β] [LT β] [DecidableLT β] (f : α → 
       apply insertCanonical_not_nil f x (canonicalize f xs)
       exact h₁
 
-theorem canonicalize_not_nil [DecidableEq β] [LT β] [DecidableLT β] (f : α → β) (xs : List α) :
+public theorem canonicalize_not_nil [DecidableEq β] [LT β] [DecidableLT β] (f : α → β) (xs : List α) :
   xs ≠ [] ↔ (canonicalize f xs) ≠ []
 := by
   constructor
@@ -331,14 +367,19 @@ theorem canonicalize_not_nil [DecidableEq β] [LT β] [DecidableLT β] (f : α �
     intro h₀
     cases xs <;> simp only [ne_eq, reduceCtorEq, not_false_eq_true, not_true_eq_false] at *
 
-theorem canonicalize_cons [LT β] [DecidableLT β] (f : α → β) (xs : List α) (a : α) :
+public theorem canonicalize_cons [LT β] [DecidableLT β] (f : α → β) (xs : List α) (a : α) :
   canonicalize f xs = canonicalize f ys → canonicalize f (a :: xs) = canonicalize f (a :: ys)
 := by
   intro h₁
   unfold canonicalize
   simp [h₁]
 
-theorem canonicalize_sortedBy [LT β] [StrictLT β] [DecidableLT β] (f : α → β) (xs : List α) :
+public theorem canonicalize_singleton [LT β] [DecidableLT β] (f : α → β) (x : α) :
+  canonicalize f [x] = [x]
+:= by
+  simp [canonicalize, insertCanonical]
+
+public theorem canonicalize_sortedBy [LT β] [StrictLT β] [DecidableLT β] (f : α → β) (xs : List α) :
   SortedBy f (canonicalize f xs)
 := by
   induction xs
@@ -348,7 +389,7 @@ theorem canonicalize_sortedBy [LT β] [StrictLT β] [DecidableLT β] (f : α →
     apply insertCanonical_sortedBy
     exact ih
 
-theorem sortedBy_implies_canonicalize_eq [LT β] [StrictLT β] [DecidableLT β] {f : α → β} {xs : List α} :
+public theorem sortedBy_implies_canonicalize_eq [LT β] [StrictLT β] [DecidableLT β] {f : α → β} {xs : List α} :
   SortedBy f xs → (canonicalize f xs) = xs
 := by
   intro h₁
@@ -360,7 +401,7 @@ theorem sortedBy_implies_canonicalize_eq [LT β] [StrictLT β] [DecidableLT β] 
       specialize ih h₁
       simp [ih, insertCanonical, h₂]
 
-theorem canonicalize_subseteq [LT β] [StrictLT β] [DecidableLT β] (f : α → β) (xs : List α) :
+public theorem canonicalize_subseteq [LT β] [StrictLT β] [DecidableLT β] (f : α → β) (xs : List α) :
   xs.canonicalize f ⊆ xs
 := by
   induction xs <;> simp only [canonicalize, Subset.refl]
@@ -372,7 +413,7 @@ theorem canonicalize_subseteq [LT β] [StrictLT β] [DecidableLT β] (f : α →
     simp only [subset_cons_self]
 
 /-- Corollary of `canonicalize_subseteq` -/
-theorem in_canonicalize_in_list [LT β] [StrictLT β] [DecidableLT β] {f : α → β} {x : α} {xs : List α} :
+public theorem in_canonicalize_in_list [LT β] [StrictLT β] [DecidableLT β] {f : α → β} {x : α} {xs : List α} :
   x ∈ xs.canonicalize f → x ∈ xs
 := by
   intro h₁
@@ -385,7 +426,7 @@ Note that `canonicalize_equiv` does not hold for all functions `f`.
 To see why, consider xs = [(1, false), (1, true)], f = Prod.fst.
 Then `canonicalize f xs = [(1, false)] !≡ xs`.
 -/
-theorem canonicalize_equiv [LT α] [StrictLT α] [DecidableLT α] (xs : List α) :
+public theorem canonicalize_equiv [LT α] [StrictLT α] [DecidableLT α] (xs : List α) :
   xs ≡ canonicalize id xs
 := by
   induction xs
@@ -403,7 +444,7 @@ theorem canonicalize_equiv [LT α] [StrictLT α] [DecidableLT α] (xs : List α)
 Note that `equiv_implies_canonical_eq` does not hold for all functions `f`.
 To see why, consider the `example` immediately below this.
 -/
-theorem equiv_implies_canonical_eq [LT α] [StrictLT α] [DecidableLT α] (xs ys : List α) :
+public theorem equiv_implies_canonical_eq [LT α] [StrictLT α] [DecidableLT α] (xs ys : List α) :
   xs ≡ ys → (canonicalize id xs) = (canonicalize id ys)
 := by
   intro h₁
@@ -435,7 +476,7 @@ example :
   simp [List.Equiv]
   decide
 
-theorem canonicalize_idempotent {α β} [LT β] [StrictLT β] [DecidableLT β] (f : α → β) (xs : List α) :
+public theorem canonicalize_idempotent {α β} [LT β] [StrictLT β] [DecidableLT β] (f : α → β) (xs : List α) :
   canonicalize f (canonicalize f xs) = canonicalize f xs
 := sortedBy_implies_canonicalize_eq (canonicalize_sortedBy f xs)
 
@@ -448,7 +489,7 @@ Then `(canonicalize f xs).filter p = []` but `(xs.filter p).canonicalize f = [(1
 #eval (canonicalize Prod.fst [(1, false), (1, true)]).filter Prod.snd
 #eval ([(1, false), (1, true)].filter Prod.snd).canonicalize Prod.fst
 -/
-theorem canonicalize_id_filter {α} [LT α] [StrictLT α] [DecidableLT α] (p : α → Bool) (xs : List α) :
+public theorem canonicalize_id_filter {α} [LT α] [StrictLT α] [DecidableLT α] (p : α → Bool) (xs : List α) :
   (canonicalize id xs).filter p = (xs.filter p).canonicalize id
 := by
   have h₁ : (canonicalize id xs).filter p ≡ xs.filter p := by
@@ -461,7 +502,7 @@ theorem canonicalize_id_filter {α} [LT α] [StrictLT α] [DecidableLT α] (p : 
     (canonicalize_sortedBy id (filter p xs))
     (Equiv.trans h₁ h₂)
 
-theorem canonicalize_preserves_forallᵥ {α β γ} [LT α] [StrictLT α] [DecidableLT α] (p : β → γ → Prop) (kvs₁ : List (α × β)) (kvs₂ : List (α × γ)) :
+public theorem canonicalize_preserves_forallᵥ {α β γ} [LT α] [StrictLT α] [DecidableLT α] (p : β → γ → Prop) (kvs₁ : List (α × β)) (kvs₂ : List (α × γ)) :
   List.Forallᵥ p kvs₁ kvs₂ →
   List.Forallᵥ p (List.canonicalize Prod.fst kvs₁) (List.canonicalize Prod.fst kvs₂)
 := by
@@ -474,7 +515,7 @@ theorem canonicalize_preserves_forallᵥ {α β γ} [LT α] [StrictLT α] [Decid
     have h₄ := canonicalize_preserves_forallᵥ p tl₁ tl₂ h₃
     apply insertCanonical_preserves_forallᵥ h₂ h₄
 
-theorem canonicalize_of_map_fst {α β γ} [LT α] [StrictLT α] [DecidableLT α] (xs : List (α × β)) (f : β → γ) :
+public theorem canonicalize_of_map_fst {α β γ} [LT α] [StrictLT α] [DecidableLT α] (xs : List (α × β)) (f : β → γ) :
   List.canonicalize Prod.fst (List.map (Prod.map id f) xs) =
   List.map (Prod.map id f) (List.canonicalize Prod.fst xs)
 := by
